#   Licensed to the NLP2RDF project under one or more
#   contributor license agreements.  See the NOTICE file distributed with
#   this work for additional information regarding copyright ownership.
#   The ASF licenses this file to You under the Apache License, Version 2.0
#   (the "License"); you may not use this file except in compliance with
#   the License.  You may obtain a copy of the License at
#
#        http://www.apache.org/licenses/LICENSE-2.0
#
#   Unless required by applicable law or agreed to in writing, software
#   distributed under the License is distributed on an "AS IS" BASIS,
#   WITHOUT WARRANTIES OR CONDITIONS OF ANY KIND, either express or implied.
#   See the License for the specific language governing permissions and
#   limitations under the License.


@prefix rdf: <http://www.w3.org/1999/02/22-rdf-syntax-ns#> .
@prefix rdfs: <http://www.w3.org/2000/01/rdf-schema#> .
@prefix owl: <http://www.w3.org/2002/07/owl#> .
@prefix xsd: <http://www.w3.org/2001/XMLSchema#> .
@prefix dcterms: <http://purl.org/dc/terms/> .
@prefix foaf: <http://xmlns.com/foaf/0.1/> .
@prefix nif: <http://persistence.uni-leipzig.org/nlp2rdf/ontologies/nif-core#> .
@prefix nerd: <http://nerd.eurecom.fr/ontology#> .
@prefix itsrdf: <http://www.w3.org/2005/11/its/rdf#> .
@prefix prov: <http://www.w3.org/ns/prov#> .
@prefix skosxl: <http://www.w3.org/2008/05/skos-xl#> .
@prefix vs: <http://www.w3.org/2003/06/sw-vocab-status/ns#> .
@prefix vann: <http://purl.org/vocab/vann/> .
@prefix oa: <http://www.w3.org/ns/oa#> .
@prefix marl: <http://purl.org/marl/ns#> .
@prefix fise: <http://fise.iks-project.eu/ontology/> .

<http://persistence.uni-leipzig.org/nlp2rdf/ontologies/nif-core#> 
    a owl:Ontology ;
    rdfs:label "NIF 2.0 Core Ontology"@en ;
    vann:preferredNamespacePrefix "nif" ;
    vann:preferredNamespaceUri "http://persistence.uni-leipzig.org/nlp2rdf/ontologies/nif-core#" ;
    vann:changes <https://github.com/NLP2RDF/persistence.uni-leipzig.org/commits/master/ontologies/nif-core> ;
    rdfs:comment """
# Disclaimer
This ontology is part of the NLP2RDF project and provided as part of the NLP Interchange Format Version 2.0 under CC-BY license as well as Apache 2.0. 
More documentation is available at the NIF/NLP2RDF overview page: http://persistence.uni-leipzig.org/nlp2rdf/
# Relation to the FISE ontology
FISE is an ontology originated from Apache Stanbol and found here: http://fise.iks-project.eu/ontology/
The ontology was compatible and useful and we just included it here.

# Ontolgy setup
This ontology is split in three parts:
* a terminological model (containing rdfs:comment, rdfs:label, rdfs:subClassOf, rdfs:subPropertyOf, rdfs:range and rdfs:domain statements)
* an inference model (containing owl:TransitiveProperty, owl:hasKey)
* a validation model (containing owl:FunctionalProperty, owl:DisjointWith)
This is also the reason for the three rdfs:isDefinedBy properties.
The ontology is developed at GitHub: https://github.com/NLP2RDF/persistence.uni-leipzig.org#readme (also older versions are there).
You can find RDF/XML serializations online, but we only edit the turtle file in the repository. 

# Other Ontologies
NLP2RDF works together with several other projects, that make very good ontologies, which we are reusing for NIF 2.0. Please import them, if necessary:
* http://purl.org/olia
* http://www.w3.org/2005/11/its/rdf#

# Examples
At the end of this ontology we provide an example. 
"""@en ;
    rdfs:isDefinedBy <http://persistence.uni-leipzig.org/nlp2rdf/ontologies/nif-core/version-1.0/nif-core.ttl> ;
    rdfs:isDefinedBy <http://persistence.uni-leipzig.org/nlp2rdf/ontologies/nif-core/version-1.0/nif-core-inf.ttl> ;
    rdfs:isDefinedBy <http://persistence.uni-leipzig.org/nlp2rdf/ontologies/nif-core/version-1.0/nif-core-val.ttl> ;
    owl:versionInfo "see GitHub for all version https://github.com/NLP2RDF/persistence.uni-leipzig.org " ;
    owl:versionIRI <http://persistence.uni-leipzig.org/nlp2rdf/ontologies/nif-core/version-1.0/nif-core.ttl> ;
    dcterms:license <http://www.apache.org/licenses/LICENSE-2.0> ;
    dcterms:license <http://creativecommons.org/licenses/by/3.0/> .

###################
# Base Classes
###################

nif:Context
    a owl:Class ;
    vs:term_status "1.0.0" ;
    vs:changelog """1.0.0: Introduced stable version, linking to the ISWC In Use publication for documentation.""" ;
    rdfs:label "Context"@en ;
    rdfs:comment """ see http://svn.aksw.org/papers/2013/ISWC_NIF/public.pdf """ ;
    rdfs:subClassOf nif:String .
    
nif:String
    a owl:Class ;
    vs:term_status "1.0.0" ;
    vs:changelog """1.0.0: Introduced stable version, linking to the ISWC In Use publication for documentation.""" ;
    rdfs:label "String"@en ;
    rdfs:subClassOf nif:Annotation ;
    rdfs:comment """ see http://svn.aksw.org/papers/2013/ISWC_NIF/public.pdf This is a subclass of Annotation, because it "annotates" strings for example with begin and end index. It is also very similar to fise:TextAnnotation"""@en .
    
nif:Annotation
    a owl:Class ;
    vs:term_status "unstable" ;
    rdfs:label "Annotation"@en ;
    rdfs:comment """This class is an individual used in the NIF-Stanbol profile and can be a URN """@en .

    
nif:URIScheme 
    a owl:Class ;
    vs:term_status "unstable" ;
    rdfs:label "URI Scheme"@en ;
    rdfs:comment "A URI Scheme for NIF, subclasses need to define guidelines on the URI Scheme as well as the text it refers to. This class is just to keep some order, please don't serialize." ;
    rdfs:subClassOf nif:String .
    

nif:Structure
    a owl:Class ;
    vs:term_status "unstable" ;
    rdfs:label "Structure"@en ;
    rdfs:comment """A structure is a more or less arbitrary label for a partitioning of a string. We do not follow a strict approach for what a word, phrase, sentence, title, paragraph is. These labels enable the definition processes for tool chains, e.g. tool analyses nif:Paragraph and calculates term frequency. """ ;
    rdfs:subClassOf nif:String .
   
    
# experimental
nif:HTMLString
    a owl:Class ;
    vs:term_status "unstable" ;
    vs:term_status "experimental" ;
    rdfs:label "HTML String"@en ;
    rdfs:comment """experimental, a subspecialisation of String (a string with HTML markup). """@en ;
    rdfs:subClassOf nif:String .
    
###################
# Basic Properties
###################    

nif:referenceContext
    a owl:ObjectProperty ;
    vs:term_status "1.0.0" ;
    vs:changelog """1.0.0: Introduced stable version.""" ;
    rdfs:label "reference context"@en ;
    rdfs:comment """The reference text (called nif:Context) a nif:String occurs in.  
    Each String instance must have exactly one reference context. 
    Instances of nif:Context have itself as reference context (see also nif-core-inf.ttl)  . 
    This property is functional in the validation model (nif-core-val.ttl)."""@en ;
    rdfs:domain nif:String ;
    rdfs:range nif:Context .

nif:isString
    a owl:DatatypeProperty ;
    vs:term_status "1.0.0" ;
    vs:changelog """1.0.0: Introduced stable version.""" ;
    rdfs:label "is string"@en ; 
    rdfs:comment """The reference text as rdf:Literal for this nif:Context resource.  
    NIF highly recommends to always include the reference text (i.e. the context) as an rdf:Literal.
    Note, that the isString property is *the* place to keep the string itself in RDF.
    All other nif:Strings and nif:URISchemes relate to the text of this property to calculate character position and indices. """@en ;
	rdfs:subPropertyOf nif:anchorOf ;
    rdfs:domain nif:Context .

    
nif:beginIndex
    a owl:DatatypeProperty ;
    vs:term_status "1.0.0" ;
    vs:changelog """1.0.0: Introduced stable version.""" ;
    rdfs:label "begin index"@en ;
    rdfs:comment """The begin index of a character range as defined in http://tools.ietf.org/html/rfc5147#section-2.2.1 and http://tools.ietf.org/html/rfc5147#section-2.2.2, measured as the gap between two characters, starting to count from 0 (the position before the first character of a text). 
    Example: Index "2" is the postion between "Mr" and "."  in "Mr. Sandman".
    Note: RFC 5147 is re-used for the definition of character ranges. RFC 5147 is assuming a text/plain MIME type. NIF builds upon Unicode and is content agnostic. 
    Requirement (1): This property has the same value the "Character position" of RFC 5147 and it must therefore be an xsd:nonNegativeInteger .  
    Requirement (2): The index of the subject string MUST be calculated relative to the nif:referenceContext of the subject. If available, this is the rdf:Literal of the nif:isString property.""" ;
    # still being discussed:
    # rdfs:subPropertyOf oa:start ;
    # rdfs:range <http://www.w3.org/2001/XMLSchema#nonNegativeInteger> ;
    rdfs:domain nif:String .

nif:endIndex
    a owl:DatatypeProperty ;
    vs:term_status "1.0.0" ;
    vs:changelog """1.0.0: Introduced stable version.""" ;
    rdfs:label "end index"@en ;
    rdfs:comment """The end index of a character range as defined in http://tools.ietf.org/html/rfc5147#section-2.2.1 and http://tools.ietf.org/html/rfc5147#section-2.2.2, measured as the gap between two characters, starting to count from 0 (the position before the first character of a text). 
    Example: Index "2" is the postion between "Mr" and "."  in "Mr. Sandman".
    Note: RFC 5147 is re-used for the definition of character ranges. RFC 5147 is assuming a text/plain MIME type. NIF builds upon Unicode and is content agnostic. 
    Requirement (1): This property has the same value the "Character position" of RFC 5147 and it must therefore be an xsd:nonNegativeInteger .  
    Requirement (2): The index of the subject string MUST be calculated relative to the nif:referenceContext of the subject. If available, this is the rdf:Literal of the nif:isString property.""" ;
    # still being discussed:
    # rdfs:subPropertyOf oa:end ;
    # rdfs:range <http://www.w3.org/2001/XMLSchema#nonNegativeInteger> ;
    rdfs:domain nif:String .
    
nif:anchorOf
    a owl:DatatypeProperty ;
    vs:term_status "testing" ;
    vs:term_status "optional" ;
    rdfs:label "anchor of"@en ;
    rdfs:comment "The string, which the uri is representing as an RDF Literal. Some use cases require this property, as it is necessary for certain sparql queries. " ;
    rdfs:domain nif:String .

nif:sourceUrl
    a owl:ObjectProperty ;
    vs:term_status "testing" ;
    rdfs:label "source URL"@en ;	
    rdfs:comment "The URL the context was extracted from, e.g. the blog or news article url. Doesn't matter whether it is HTML or XML or plain text. rdfs:range is foaf:Document, if the string comes form another NIF String, please use nif:wasConvertedFrom"@en ;
    rdfs:domain nif:Context .

nif:wasConvertedFrom
    a owl:ObjectProperty ;
    vs:term_status "testing" ;
    rdfs:label "was converted from"@en ;	
    rdfs:comment """This property should be used, when mapping one NIF String URIScheme to another.
    It mainly is used to provide provenance during a conversion process, e.g. when removing tags from XHTML and then linking XPath URIs to NIF index based URIs (e.g.  RFC 5147 with char=x,y).
    An example of the usage of this property can be found here: http://www.w3.org/TR/its20/#conversion-to-nif
    """@en ;
    rdfs:subPropertyOf prov:wasDerivedFrom ;
    rdfs:domain nif:String ;
    rdfs:range nif:String .
    
nif:broaderContext
    a owl:ObjectProperty ;
    vs:term_status "testing" ;
    rdfs:label "broader Context"@en ;	
    rdfs:comment "This property should be used to express that one Context is contained in another Context, e.g. several sentences of a document are modelled indivudally and refer to the broader context of the whole document."@en ;
    rdfs:domain nif:Context ;
    rdfs:range nif:Context .
    
nif:narrowerContext
    a owl:ObjectProperty ;
    vs:term_status "testing" ;
    rdfs:label "narrower Context"@en ;	
    rdfs:comment "The inverse of nif:narrowerContext"@en ;
    rdfs:domain nif:Context ;
    rdfs:range nif:Context .

nif:before
    a owl:DatatypeProperty ;
    vs:term_status "testing" ;
    rdfs:label "before"@en ;
    rdfs:comment "For each string you can include a snippet (e.g. 10-40 characters of text), that occurs immediately before the subject string." ;
    rdfs:domain nif:String .

nif:after
    a owl:DatatypeProperty ;
    vs:term_status "testing" ;
    rdfs:label "after"@en ;
    rdfs:comment "For each string you can include a snippet (e.g. 10-40 characters of text), that occurs immediately after the subject string." ;
    rdfs:domain nif:String .

nif:head a owl:DatatypeProperty ;
    vs:term_status "unstable" ;
    rdfs:label "head"@en ;
     rdfs:comment """
      The first few chars of the nif:anchorOf. Typically used if the nif:anchorOf
      is to long for inclusion as RDF literal.
    """@en ;
    rdfs:domain nif:String .
    
nif:tail
    vs:term_status "unstable" ;
    rdfs:label "tail"@en ;
    rdfs:comment """
      The last few chars of the nif:anchorOf. Typically used if the nif:anchorOf
      is to long for inclusion as RDF literal.
    """@en ;
    rdfs:domain nif:String .
    
nif:contextAsLiteral    
    vs:term_status "unstable" ;
    rdfs:label "contextAsLiteral"@en ;
    rdfs:comment """
      The string that the nif:anchorOf is embedded in. FILTER ( strlen (nif:referenceContext [ nif:isString ] ) ) 
    """@en ;
    rdfs:domain nif:String .

###################
# properties for extensions
###################

nif:contextAsLiteral    
	a owl:DatatypeProperty ;
    vs:term_status "unstable" ;
    rdfs:label "contextAsLiteral"@en ;
    rdfs:comment """
      The string that the nif:anchorOf is embedded in. FILTER ( strlen (nif:referenceContext [ nif:isString ] ) ) 
    """@en ;
    rdfs:domain nif:String .


nif:annotation    
	a owl:ObjectProperty ;
    vs:term_status "unstable" ;
    rdfs:label "annotation"@en ;
    rdfs:comment """
      see Towards Web-Scale Collaborative Knowledge Extraction  http://svn.aksw.org/papers/2012/PeoplesWeb/public_preprint.pdf‎ page 5 .
    """@en ;
    rdfs:domain nif:Annotation .

nif:literalAnnotation    
	a owl:DatatypeProperty ;
    vs:term_status "unstable" ;
    rdfs:label "literalAnnotation"@en ;
    rdfs:comment """
      see Towards Web-Scale Collaborative Knowledge Extraction  http://svn.aksw.org/papers/2012/PeoplesWeb/public_preprint.pdf‎ page 5 .
    """@en ;
    rdfs:domain nif:Annotation .
    
nif:classAnnotation   
	a owl:AnnotationProperty ;
    vs:term_status "unstable" ;
    rdfs:label "classAnnotation"@en ;
    rdfs:comment """
      see Towards Web-Scale Collaborative Knowledge Extraction  http://svn.aksw.org/papers/2012/PeoplesWeb/public_preprint.pdf‎ page 5 .
    """@en ;
    rdfs:domain nif:Annotation .

###################
# URI Schemes
###################

nif:RFC5147String
    a owl:Class ;
    vs:term_status "1.0.0" ;
    vs:changelog """1.0.0: Introduced stable version.""" ;
    rdfs:label "RFC 5147 string"@en ;
    rdfs:comment "cf. http://tools.ietf.org/html/rfc5147 " ;
    rdfs:subClassOf nif:URIScheme .

nif:ContextHashBasedString
    a owl:Class ;
    vs:term_status "1.0.0" ;
    vs:changelog """1.0.0: Introduced stable version.""" ;
    rdfs:label "Context hash based string"@en ;
    rdfs:comment " cf. https://www.google.de/search?q=Linked-Data+Aware+URI+Schemes+for+Referencing+Text" ;
    rdfs:subClassOf nif:URIScheme .
    
nif:OffsetBasedString
    a owl:Class ;
    vs:term_status "stable" ;
    vs:term_status "deprecated" ;
    rdfs:label "Offset based string"@en ;
    rdfs:comment "cf. https://www.google.de/search?q=Linked-Data+Aware+URI+Schemes+for+Referencing+Text" ;
    rdfs:subClassOf nif:URIScheme .
    
nif:ArbitraryString
    a owl:Class ;
    vs:term_status "unstable" ;
    rdfs:label "Text Annotation"@en ;
    rdfs:comment """An abitrary URI (e.g. a URN) for an arbitrary string of the context. This is exactly the same as TextAnnotations are currently implemented in Stanbol."""@en ;
    rdfs:subClassOf nif:URIScheme .
    
#experimental
nif:OccuringWord
    a owl:Class ;
    vs:term_status "unstable" ;
    rdfs:label "Occuring String"@en ;
	rdfs:comment """Instances of this class represent all occuring words with a matching string within the same context. The pattern for this scheme is 'occ_'+urlencode($anchorOf) . If the text is tokenizedd with nif:Word, instances of this class would be the same as the combination of all instances, that have the same nif:anchorOf and the same nif:referenceContext. It is a scheme to refer to all tokens with the exact same string in one text. If such a URI is used, it implies, that the word occurs at least once in the given context. Otherwise nif:LabelString should be used. """@en ;
    rdfs:subClassOf nif:String .


nif:LabelString
    a owl:Class ;
    vs:term_status "unstable" ;
    vs:term_status "experimental" ;
    rdfs:label "Label String"@en ;
	rdfs:comment """Instances of this class represent a label independent from any context. This class is a subClassOf skosxl:Label, but disjoint with nif:String (see nif-core-val.ttl). We included this class in nif-core, because we are proposing the following scheme for it: 'label_'+urlencode($term).   """@en ;
    rdfs:subClassOf skosxl:Label .

#experimental
nif:XPathString 
    a owl:Class ;
    vs:term_status "unstable" ;
    vs:term_status "experimental" ;
    rdfs:label "XPath string"@en ;
#   rdfs:comment """ TODO """ ;
    rdfs:subClassOf nif:HTMLString .
  


    
###################
# Structure
###################

nif:Word
    a owl:Class ;
    vs:term_status "testing" ;  
    rdfs:label "word"@en ;
    rdfs:comment """
    Assigning this class to a nif:String This class has definitory 
    A string that can be considered a word or a punctuation mark, the sentence 'He enters the room.' for example has 5 words. In general, the division into nif:Word is done by a tokenizer. Instances of this class are defined as a string, that is a 'meaningful' unit of characters. The class is not descriptive, but prescriptive. All NIF tools are supposed to either honor the current assignment of nif:Word or possibly correct it, if that is intended by the developer. 
    The class has not been named 'Token' as the NLP definition of 'Token' is more similar to our definition of nif:String in general, e.g. "can't" could be one, two or three tokens."""@en ;
    rdfs:subClassOf nif:Structure  .

nif:Phrase
    a owl:Class ;
    vs:term_status "testing" ;   
    rdfs:label "a Phrase"@en ;
    rdfs:comment """A nif:Phrase can be a nif:String, that is a chunk of several words or a word itself (e.g. a NounPhrase as a Named Entity). The term is underspecified and can be compatible with many defintitions of phrase. Please subClass it to specify the meaning (e.g. for Chunking or Phrase Structure Grammar). Example: ((My dog)(also)(likes)(eating (sausage))) """ ;
    rdfs:subClassOf nif:Structure  .

nif:Sentence
    a owl:Class ;
    vs:term_status "testing" ; 
    rdfs:label "a Sentence"@en ;
    rdfs:comment "a sentence." ;
    rdfs:subClassOf nif:Structure  .

nif:Paragraph
    a owl:Class ;
    vs:term_status "unstable" ;  
    rdfs:label "a Paragraph"@en ;
    rdfs:comment "a Paragraph." ;
    rdfs:subClassOf nif:Structure  .
    
nif:Title
    a owl:Class ;
    vs:term_status "unstable" ;  
    rdfs:label "title"@en ;
    rdfs:comment "a title within a text." ;
    rdfs:subClassOf nif:Structure  .
    
###################
# Structure properties
###################


###################
# String level
###################

nif:subString
    a owl:ObjectProperty ;
    vs:term_status "unstable" ;
    rdfs:label "sub string"@en ;
    rdfs:comment """This property together with nif:subString, nif:superString, and their transitive extension can be used to express that one string is contained in another one. Examples: "a" nif:subString "apple" , "apple" nif:subString "apple".  The transitivity axioms are included in nif-core-inf.ttl and need to be included separately to keep a low reasoning profile. They are modeled after skos:broader and skos:broaderTransitive"""@en ;
    rdfs:domain nif:String ;
    rdfs:range nif:String ;
    rdfs:subPropertyOf nif:subStringTrans .

nif:subStringTrans
    a owl:ObjectProperty  ;
    vs:term_status "unstable" ;
    rdfs:label "transitive version of subString"@en ;
    rdfs:comment "see nif:subString"@en ;
    rdfs:domain nif:String ;
    rdfs:range nif:String .

nif:superString
    a owl:ObjectProperty ;
    vs:term_status "unstable" ;
    rdfs:label "super String"@en ;
    rdfs:comment "see nif:subString"@en ;
    rdfs:domain nif:String ;
    rdfs:range nif:String ;
    rdfs:subPropertyOf nif:superStringTrans .

nif:superStringTrans
    a owl:ObjectProperty ;
    vs:term_status "unstable" ;
    rdfs:label "transitive version of superString"@en ;
    rdfs:comment "see nif:subString"@en ;
    rdfs:domain nif:String ;
    rdfs:range nif:String .

###############
# Sentence level
###############

nif:nextSentence
    a owl:ObjectProperty ;
    vs:term_status "unstable" ;
    rdfs:comment """This property (and nif:previousSentence, nif:nextWord, nif:previousWord and their transitive extension) can be used to make resources of nif:Sentence and nif:Word traversable, it can not be assumed that no gaps or whitespaces between sentences or words exist, i.e. string adjacency is not mandatory. The transitivity axioms are included in nif-core-inf.ttl and need to be included separately to keep a low reasoning profile. They are modeled after skos:broader and skos:broaderTransitive"""@en ;
    rdfs:domain nif:Sentence ;
    rdfs:range nif:Sentence ;
    rdfs:subPropertyOf nif:nextSentenceTrans .

nif:nextSentenceTrans
    a owl:ObjectProperty ;
    vs:term_status "unstable" ;
    rdfs:comment "see nif:nextSentence"@en ;
    rdfs:domain nif:Sentence ;
    rdfs:range nif:Sentence  .

nif:previousSentence
	a owl:ObjectProperty ;
	vs:term_status "unstable" ;
    rdfs:comment "see nif:nextSentence"@en ;
    rdfs:domain nif:Sentence ;
    rdfs:range nif:Sentence ;
    rdfs:subPropertyOf nif:previousSentenceTrans .

nif:previousSentenceTrans
    a owl:ObjectProperty ;
    vs:term_status "unstable" ;
    rdfs:comment "see nif:nextSentence"@en ;
    rdfs:domain nif:Sentence ;
    rdfs:range nif:Sentence .
    
    
nif:word
    a owl:ObjectProperty ;
    vs:term_status "unstable" ;
    rdfs:label "has word"@en ;
    rdfs:comment "This property links sentences to their words."@en ;
    rdfs:domain nif:Sentence ;
    rdfs:range nif:Word .

nif:firstWord
    a owl:ObjectProperty ;
    vs:term_status "unstable" ;
    rdfs:label "has first word"@en ;
    rdfs:comment "This property links sentences to their first word."@en ;
    rdfs:domain nif:Sentence ;
    rdfs:range nif:Word ;
    rdfs:subPropertyOf nif:word .

nif:lastWord
    a owl:ObjectProperty ;
    vs:term_status "unstable" ;
    rdfs:label "has first word"@en ;
    rdfs:comment "This property links sentences to their last word."@en ;
    rdfs:domain nif:Sentence ;
    rdfs:range nif:Word ;
    rdfs:subPropertyOf nif:word .
    
###############
# Word level
###############

nif:occurrence
    a owl:ObjectProperty ;
    vs:term_status "unstable" ;
    rdfs:comment "This property links a URI of type OccuringWord to other nif:String, that occur in the same context." ;
    rdfs:domain nif:OccuringWord ;
    rdfs:range nif:String .

nif:sentence
    a owl:ObjectProperty ;
    vs:term_status "unstable" ;
    rdfs:comment "This property links words to their sentence." ;
    rdfs:domain nif:Word ;
    rdfs:range nif:Sentence .

nif:nextWord
    a owl:ObjectProperty ;
    vs:term_status "unstable" ;
    rdfs:comment "see nif:nextSentence"@en ;
    rdfs:domain nif:Word ;
    rdfs:range nif:Word ;
    rdfs:subPropertyOf nif:nextWordTrans .
 

nif:nextWordTrans
    a owl:ObjectProperty ;
    vs:term_status "unstable" ;
    rdfs:comment "see nif:nextSentence"@en ;
    rdfs:domain nif:Word ;
    rdfs:range nif:Word .
    

nif:previousWord
    a owl:ObjectProperty ;
    vs:term_status "unstable" ;
    rdfs:comment "see nif:nextSentence"@en ;
    rdfs:domain nif:Word ;
    rdfs:range nif:Word ;
    rdfs:subPropertyOf nif:previousWordTrans .

nif:previousWordTrans
    a owl:ObjectProperty ;
    vs:term_status "unstable" ;
    rdfs:comment "see nif:nextSentence"@en ;
    rdfs:domain nif:Word ;
    rdfs:range nif:Word .

###############
# Properties for common annotations
###############

###############
# lemma, stem
###############

nif:lemma
	a owl:DatatypeProperty ;
	vs:term_status "testing" ;  
	rdfs:label "lemma"@en ;
	rdfs:comment "The lemma(s) of the nif:String."@en ;
	rdfs:domain nif:String ;
	rdfs:range xsd:string .

nif:stem
	a owl:DatatypeProperty ;
	vs:term_status "testing" ;  
	rdfs:label "stem"@en ;
	rdfs:comment "The stem(s) of the nif:String."@en ;
	rdfs:domain nif:String ;
	rdfs:range xsd:string .



###############
# Part of Speech (POS) Tags
###############

nif:oliaLink
    a owl:ObjectProperty ;
    vs:term_status "testing" ; 
    rdfs:label "OLiA link"@en ;
    rdfs:comment """This property links a string to a URI from one of the OLiA Annotation model, e.g. http://purl.org/olia/penn.owl#NNP """@en ;
    ## rdfs:range TODO ;
    rdfs:domain nif:String .
    
nif:oliaLinkConf
    a owl:DatatypeProperty ;
    vs:term_status "unstable" ; 
    rdfs:label "confidence of OLiA link" ;
    rdfs:comment "The confidence is relative to the tool and can be between 0.0 and 1.0 "@en ;
    rdfs:range xsd:decimal ;
    rdfs:domain nif:String .
    
nif:oliaCategory
    a owl:AnnotationProperty ;
    vs:term_status "testing" ; 
    rdfs:label "OLiA Category"@en ;
    rdfs:comment """This property links a string to the OLiA Reference model. It provides a direct link for querying, thus it is an optimization. """@en ;
    rdfs:domain nif:String . 

nif:oliaCategoryConf
    a owl:DatatypeProperty ;
    vs:term_status "unstable" ; 
    rdfs:label "confidence of OLiA category" ;
    rdfs:comment "The confidence is relative to the tool and can be between 0.0 and 1.0 "@en ;
    rdfs:range xsd:decimal ;
    rdfs:domain nif:String .

# use only, if no other option is available:
nif:posTag
	a owl:DatatypeProperty ;
	vs:term_status "discouraged";
	rdfs:label "Part of speech tag"@en ;
	rdfs:comment "To include the pos tag as it comes out of the NLP tool as RDF Literal. This property is discouraged to use alone, please use oliaLink and oliaCategory.  " ;
	rdfs:domain nif:String ;
	rdfs:range xsd:string .

###################
# Lexical and Corpus Level
###################  

nif:ContextOccurrence a owl:Class . #nif:URIScheme .
nif:NormalizedContextOccurrence a owl:Class . #nif:URIScheme .
nif:CollectionOccurrence a owl:Class . #nif:URIScheme .
nif:NormalizedCollectionOccurrence a owl:Class . #nif:URIScheme .

###################
# Machine Learning
###################  

nif:class 
	rdfs:label "class";
	vs:term_status "unstable" ; 
	rdfs:comment """A simple annotation for machine learning purposes. The object can be anything, e.g. the literal "A. PRESS: Reportage" from brown or any URI.  """@en ;
	a owl:AnnotationProperty .

###############
# NamedEntity
###############


###############
# Sentiment
###############    

nif:sentimentValue 
	rdfs:label "sentiment value";
	vs:term_status "unstable" ; 
	rdfs:comment """Between -1 negative and 1 positive """@en ;
	rdfs:range xsd:decimal ;
	a owl:DatatypeProperty .

nif:opinion 
	rdfs:label "opinion";
	vs:term_status "unstable" ; 
	rdfs:comment """This property is used to link to a marl:Opinion. We have not investigated marl, so it might be replaced. http://marl.gi2mo.org/?page_id=1#overview . InverseOf marl:extractedFrom"""@en ;
	rdfs:domain nif:String ;
	rdfs:range marl:Opinion ;
	a owl:ObjectProperty .

###############
# Classes for  Annotations and the NIF Stanbol profile. 
############### 	

nif:EntityAnnotation
    a owl:Class ;
    vs:term_status "unstable" ; 
    rdfs:label "Entity Annotation"@en ;
    rdfs:comment """This anntotation is an entity. Only usable with the Apache Stanbol profile. disjointWith nif:String and fise:TextAnnotation."""@en ;
    rdfs:subClassOf nif:Annotation .


nif:TopicAnnotation
    a owl:Class ;
    vs:term_status "unstable" ; 
    rdfs:label "A Topic Annotation"@en ;
    rdfs:comment """This anntotation is TODO:???? . Only usable with the Apache Stanbol profile. disjointWith nif:String and fise:TextAnnotation. """@en ;
    rdfs:subClassOf nif:Annotation .

nif:confidence
    a owl:DatatypeProperty ;
    vs:term_status "unstable" ; 
    rdfs:comment """The confidence of the nif:Annotation. If this property is attached to a nif:String, this property indicates the likelyness that the assigned indices and the nif:Structures are correct. If there are problems with URI minting use nif:ArbitraryString"""@en ;
    rdfs:domain nif:Annotation ;
    rdfs:label "confidence"@en ;
    rdfs:range xsd:decimal .
    
nif:extractedFrom
	vs:term_status "unstable" ; 
    a owl:ObjectProperty ;
    rdfs:comment """links a nif:String to a nif:Annotation ."""@en ;
    rdfs:domain nif:String ;
    rdfs:range [owl:unionOf (nif:TopicAnnotation  nif:EntityAnnotation ) ] ;
    rdfs:label "extracted from"@en .

###############
# Confidence
###############    
# might be moved to external
nif:ConfidenceLevel
    a owl:Class ;
    rdfs:comment """Class for the four different confidence levels defined by this ontology (introduced with STANBOL-631)"""@en ;
    rdfs:label "Confidence Level"@en .

# might be moved to external
nif:cl_ambiguous
    a nif:ConfidenceLevel ;
    rdfs:comment """Indicates that an Enhancement is ambiguous with an other one. To be used in cases where there are several possibilities but it is likelly that one of those is the correct one (e.g. Paris, Paris (Texas)).
Enhancements with this confidence value typically need some kind of manual disambiguation step (introduced by STANBOL-631)"""@en ;
    rdfs:label "ambiguous"@en .

# might be moved to external
nif:cl_certain
    a nif:ConfidenceLevel ;
    rdfs:comment "Indicates that an enhancement is very certain AND also not ambiguous. Enhancements with this confidence level can be usually accepped by annotation workfolws without manuall validation of resutls (introduced by STANBOL-631)"@en ;
    rdfs:label "Certain"@en .

# might be moved to external
nif:cl_suggestion
    a nif:ConfidenceLevel ;
    rdfs:comment """Indicates that an Enhancement is not completly certain but there are not several options (e.g. Germans -> Germany). Enhancements with this confidence level might or might not be used for automatic tagging workflows. However they can be typically suggested to users (introduced by STANBOL-631)"""@en ;
    rdfs:label "suggestion"@en .
# might be moved to external
nif:cl_uncertain
    a nif:ConfidenceLevel ;
    rdfs:comment """Indicating that an Enhancement is rather speculative. Enhancements with this confidence level can be ignored by most usecases. However they might be processed by other Enhancements Engines (introduced by STANBOL-631)"""@en ;
    rdfs:label "uncertain"@en .

nif:confidence_level
    a owl:ObjectProperty ;
    rdfs:comment "the level of confidence for this Annotation (introduced by STANBOL-631)."@en ;
    rdfs:domain nif:Annotation ;
    rdfs:label "confidence level"@en ;
    rdfs:range nif:ConfidenceLevel .


###############
# Plain text example
###############

# Stable part:
# URI for the first word
<http://nlp2rdf.lod2.eu/usecases/plaintext.txt#char=0,6> 
	a nif:RFC5147String  ;
	nif:referenceContext <http://nlp2rdf.lod2.eu/usecases/plaintext.txt#char=0,1756>  ;
	nif:beginIndex "0"^^xsd:nonNegativeInteger ;
	nif:endIndex "6"^^xsd:nonNegativeInteger ;
# unstable /testing part begins below	
	nif:anchorOf "Mexico" ;
	
	# Tokenization
	##############
	a nif:Word , nif:Phrase ;
	
	# Entity linking
	# see http://www.w3.org/TR/its20/#conversion-to-nif
	################
	itsrdf:taIdentRef  <http://dbpedia.org/resource/Mexico> ;
	itsrdf:taConfidence  "0.99"^^xsd:decimal ;
	itsrdf:taClassRef  <http://nerd.eurecom.fr/ontology#Country> ;
	
	# PartOfSpeech tagging
	######################
	nif:oliaLink <http://purl.org/olia/penn.owl#NNP> ;
	nif:oliaLinkConf "0.99"^^xsd:decimal ;
	nif:oliaCategory <http://purl.org/olia/olia.owl#Noun> ;
	nif:oliaCategory <http://purl.org/olia/olia.owl#ProperNoun> .

# the mention found in the first word
<http://dbpedia.org/resource/Mexico> 
	a <http://nerd.eurecom.fr/ontology#Country> .

## Context
<http://nlp2rdf.lod2.eu/usecases/plaintext.txt#char=0,1756> 
	a nif:RFC5147String  , nif:Context ;
	nif:beginIndex "0"^^xsd:nonNegativeInteger ;
	nif:endIndex "1756"^^xsd:nonNegativeInteger ;
	dcterms:created "2013-05-08T17:00:00Z"^^xsd:datetime ;
	nif:referenceContext <http://nlp2rdf.lod2.eu/usecases/plaintext.txt#char=0,1756>  ;
	nif:sourceUrl <http://nlp2rdf.lod2.eu/usecases/plaintext.txt>  ;
	nif:isString """Mexico expects the U.S. to accelerate the disbursement of aid to strengthen its fight against drug gangs and put back on track a $1.4 billion program that has been hamstrung by delays in recent years, Foreign Affairs Minister Patricia Espinosa said.
Espinosa, in an interview yesterday, said both U.S. President Barack Obama and Secretary of State Hillary Clinton promised to disburse $500 million this year in equipment and aid for police training as part of the bilateral Merida Initiative. Mexico expects to receive complete financing of the multi-year program by next year, she said.
"We got off to a slow start in part because this is a completely new cooperation plan," Espinosa, 52, said at Bloomberg's offices in Mexico City. "We now see that it's advancing more quickly."
(It would boring without special characters such as äöüßéèâ&auml;) .
U.S. anti-narcotics aid to Mexico suffered delays even as the death toll from President Felipe Calderon's crackdown on drug gangs surged to over 35,000 victims since he took office in 2006. Mexico received at least $480 million in U.S. aid under the program since it was signed in 2008 by Calderon and former President George W. Bush, with $380 million arriving between 2008 and 2010, according to data from the Foreign Ministry.
The shortfall in U.S. assistance has delayed the delivery of equipment including polygraph machines and Black Hawk helicopters needed to combat drug traffickers. It has also delayed the training of Mexican officials, according to the GAO report.
Until a year ago the U.S. had delivered only about 9 percent of the promised aid to Mexico and Central America because agencies involved lacked staff and funding, the U.S. Government Accountability Office said in a report in 2010.""".

